DynamoDbEncryption/dafny/DynamoDbEncryption/src/SearchInfo.dfy
@@ -274,6 +274,11 @@ module SearchableEncryptionInfo {
                       && var oldPutHistory := old(cache.History.PutCacheEntry);
                       && var newPutHistory := cache.History.PutCacheEntry;
                       && |newPutHistory| == |oldPutHistory|+1
+                      && (
+                        var storeOutput := Seq.Last(newPutHistory).output;
+                        || storeOutput.Success?
+                        || storeOutput.error.EntryAlreadyExists?
+                      )
                       && var storeInput := Seq.Last(newPutHistory).input;
                       && var storeOutput := Seq.Last(newPutHistory).output;
                       //= specification/searchable-encryption/search-config.md#get-beacon-key-materials
@@ -333,14 +338,11 @@ module SearchableEncryptionInfo {
         var keyMap :- getAllKeys(stdNames, key.value);
         var beaconKeyMaterials := rawBeaconKeyMaterials.beaconKeyMaterials.(beaconKey := None, hmacKeys := Some(keyMap));
 
+        expect now < UInt.BoundedInts.INT64_MAX - cacheTTL;
           //= specification/searchable-encryption/search-config.md#get-beacon-key-materials
           //# These materials MUST be put into the associated [Key Store Cache](#key-store-cache)
           //# with an [Expiry Time](../../submodules/MaterialProviders/aws-encryption-sdk-specification/framework/cryptographic-materials-cache.md#expiry-time)
           //# equal to now + configured [cacheTTL](#cachettl).
-        :- expect Need(
-          (now as int + cacheTTL as int) < UInt.INT64_MAX_LIMIT,
-          MP.AwsCryptographicMaterialProvidersException(message := "INT64 Overflow when putting cache entry.")
-        );
         var putCacheEntryInput:= MP.PutCacheEntryInput(
           identifier := identifier,
           materials := MP.Materials.BeaconKey(beaconKeyMaterials),
